IMPminus_TM/WHILE_TM/WHILE_TM.thy
@@ -1,541 +1,626 @@
 theory WHILE_TM
-  imports "IMP_Minus.AExp" "IMP_Minus.Com" "HOL-IMP.Star" Main  "IMP_Minus.Big_StepT"
-   Cook_Levin.Basics Cook_Levin.Combinations
+  imports "IMP_Minus.AExp" "IMP_Minus.Com" "HOL-IMP.Star" Main  "IMP_Minus.Big_StepT"  "IMPminus_State_TM_Tape_List"
+   Cook_Levin.Basics Cook_Levin.Combinations  Cook_Levin.Elementary   Cook_Levin.Arithmetic 
 begin
 
-fun count_atomExp_variable ::"atomExp \<Rightarrow>vname set" where
-"count_atomExp_variable (N val) ={}"| 
-"count_atomExp_variable (V vname) ={vname}"
+fun carry_minus :: "symbol list \<Rightarrow> symbol list \<Rightarrow> nat \<Rightarrow> symbol" where
+  "carry_minus xs ys 0 = \<triangleright>" |
+  "carry_minus xs ys (Suc i) = (if (todigit (digit xs i) < todigit (digit ys i) + todigit (carry_minus xs ys i)) then \<one> else \<zero>)"
 
-fun count_aexp_variable::"aexp \<Rightarrow>vname set" where
-"count_aexp_variable (A a) =count_atomExp_variable a "|
-"count_aexp_variable  (Plus a b)=(count_atomExp_variable a)\<union>(count_atomExp_variable b)" |
-"count_aexp_variable  (Sub a b)=(count_atomExp_variable a)\<union>(count_atomExp_variable b)" |
-"count_aexp_variable (Parity a) =count_atomExp_variable a "|
-"count_aexp_variable  (RightShift a) =count_atomExp_variable a "              
+definition minusdigit :: "symbol list \<Rightarrow> symbol list \<Rightarrow> nat \<Rightarrow> symbol" where
+  "minusdigit xs ys i \<equiv> tosym ((todigit (digit xs i) + todigit (digit ys i) + todigit (carry_minus xs ys i)) mod 2)"
 
-fun count_com_variable::"com \<Rightarrow>vname set" where
-"count_com_variable  SKIP ={}"|
-"count_com_variable (Assign vname a) ={vname}\<union> (count_aexp_variable a)"|
-"count_com_variable (Seq Seq1 Seq2)=(count_com_variable Seq1)\<union> (count_com_variable Seq2)"|
-"count_com_variable (If vname com1 com2) = {vname}\<union> (count_com_variable com1)\<union> (count_com_variable com2)"|
-"count_com_variable (While  vname com1) = {vname}\<union> (count_com_variable com1)"
-
-(*
-instantiation char :: linorder begin
-fun less_eq_char where "(l1::char) \<le> l2 \<longleftrightarrow> True"
-fun less_char where "(l1::char) < l2 \<longleftrightarrow> True"
-instance sorry
-end
-
-instantiation list :: (linorder) linorder begin
-fun less_eq_list where "(l1::('a::linorder) list) \<le> l2 \<longleftrightarrow> True"
-fun less_list where "(l1::('a::linorder) list) < l2 \<longleftrightarrow> True"
-instance sorry
-end
-
-fun vars_to_nat:: "com \<Rightarrow> vname \<Rightarrow> nat" where
-"vars_to_nat prog x = list (count_com_variable prog)"
-
-value "sorted_list_of_set {''a'', ''n''}"
-*)
-
-(*
-definition turing_machine :: "nat \<Rightarrow> nat \<Rightarrow> machine \<Rightarrow> bool" where
-  "turing_machine k G M \<equiv> k \<ge> 2 \<and> G \<ge> 4 \<and> (\<forall>cmd\<in>set M. turing_command k (length M) G cmd)"
-*)
-
-(*TODO : numbering every variable from 1*) 
-fun num_variable::" com \<Rightarrow> (vname \<Rightarrow> nat)" where
-"num_variable com  =(\<lambda>s. 1)"
-
-fun update_list::"nat \<Rightarrow>'a \<Rightarrow>'a list \<Rightarrow>'a list" where 
-"update_list _ _ [] =[]"|
-"update_list 0 new_ele (x#xs) =new_ele#xs"|
-"update_list (Suc n) new_ele (x#xs) =x#(update_list n new_ele xs)"
-
-fun write_bit_tape::"nat \<Rightarrow>nat \<Rightarrow>command" where
-"write_bit_tape b k=( \<lambda> symbols_read_from_tapes.
-      (
-        1, \<comment> \<open>new state\<close>
-        let len =(length symbols_read_from_tapes);
-         new_symbols_of_tapes =(update_list k (b+2) symbols_read_from_tapes);
-        directions = (replicate  (k-1) Stay)@ [Right]@(replicate  (len-k) Stay)
-          in
-       (zip new_symbols_of_tapes  directions)
-      )
-   )"
-
-(*
-definition wf_command :: "nat \<Rightarrow> nat \<Rightarrow> command \<Rightarrow> bool" where
-  "wf_command k Q cmd \<equiv> \<forall>gs. length gs = k \<longrightarrow> length (snd (cmd gs)) = k \<and> fst (cmd gs) \<le> Q"
-*)
+definition cmd_minus0 :: "tapeidx \<Rightarrow> tapeidx \<Rightarrow> command" where
+  "cmd_minus0 j1 j2 rs \<equiv>
+    (if rs ! j1 = \<box> \<and> rs ! j2 = \<box> then (if todigit(last rs) = 1 then 1 else 2) else 0 ,
+     (map (\<lambda>j.
+       if j = j1 then (rs ! j, Right)
+        else if j = j2 then (tosym (( 2+ todigit (rs ! j1) - todigit (rs ! j2) - todigit (last rs)) mod 2), Right)
+        else if j = length rs - 1 then (tosym (if todigit (rs ! j1) < todigit (rs ! j2) + todigit (last rs) then 1 else 0), Stay)
+          else (rs ! j, Stay)) [0..<length rs]))"
 
 
-fun write_end_tape::"nat \<Rightarrow>command" where
-"write_end_tape k=( \<lambda> symbols_read_from_tapes.
-      (
-        2, \<comment> \<open>new state\<close>
-        let len =(length symbols_read_from_tapes);
-         new_symbols_of_tapes =(update_list k 0 symbols_read_from_tapes);
-        directions = (replicate  (k-1) Stay)@ [Left]@(replicate  (len-k) Stay)
-          in
-       (zip new_symbols_of_tapes  directions)
-      )
-   )"
+lemma  plus_minus_mod2_eq:"a\<ge>b\<longrightarrow> (a-b) mod (2::nat)=(a+b) mod 2"
+  by (simp add: mod2_eq_if)
 
-lemma write_end_tape_wf_command:
-  (* there are K tapes in total, and we write a number n to kth tape*)
-  fixes n k K G
-  assumes "k\<ge>1" and "K\<ge>k" and "Q\<ge>4"
-  shows "wf_command K Q (write_end_tape k)"
-fun count_atomExp_variable ::"atomExp \<Rightarrow>vname set" where
-"count_atomExp_variable (N val) ={}"| 
-"count_atomExp_variable (V vname) ={vname}"
-
-fun count_aexp_variable::"aexp \<Rightarrow>vname set" where
-"count_aexp_variable (A a) =count_atomExp_variable a "|
-"count_aexp_variable  (Plus a b)=(count_atomExp_variable a)\<union>(count_atomExp_variable b)" |
-"count_aexp_variable  (Sub a b)=(count_atomExp_variable a)\<union>(count_atomExp_variable b)" |
-"count_aexp_variable (Parity a) =count_atomExp_variable a "|
-"count_aexp_variable  (RightShift a) =count_atomExp_variable a "              
-
-fun count_com_variable::"com \<Rightarrow>vname set" where
-"count_com_variable  SKIP ={}"|
-"count_com_variable (Assign vname a) ={vname}\<union> (count_aexp_variable a)"|
-"count_com_variable (Seq Seq1 Seq2)=(count_com_variable Seq1)\<union> (count_com_variable Seq2)"|
-"count_com_variable (If vname com1 com2) = {vname}\<union> (count_com_variable com1)\<union> (count_com_variable com2)"|
-"count_com_variable (While  vname com1) = {vname}\<union> (count_com_variable com1)"
-
-(*
-instantiation char :: linorder begin
-fun less_eq_char where "(l1::char) \<le> l2 \<longleftrightarrow> True"
-fun less_char where "(l1::char) < l2 \<longleftrightarrow> True"
-instance sorry
-end
-
-instantiation list :: (linorder) linorder begin
-fun less_eq_list where "(l1::('a::linorder) list) \<le> l2 \<longleftrightarrow> True"
-fun less_list where "(l1::('a::linorder) list) < l2 \<longleftrightarrow> True"
-instance sorry
-end
-
-fun vars_to_nat:: "com \<Rightarrow> vname \<Rightarrow> nat" where
-"vars_to_nat prog x = list (count_com_variable prog)"
-
-value "sorted_list_of_set {''a'', ''n''}"
-*)
-
-(*
-definition turing_machine :: "nat \<Rightarrow> nat \<Rightarrow> machine \<Rightarrow> bool" where
-  "turing_machine k G M \<equiv> k \<ge> 2 \<and> G \<ge> 4 \<and> (\<forall>cmd\<in>set M. turing_command k (length M) G cmd)"
-*)
-
-(*TODO : numbering every variable from 1*) 
-fun num_variable::" com \<Rightarrow> (vname \<Rightarrow> nat)" where
-"num_variable com  =(\<lambda>s. 1)"
-
-fun update_list::"nat \<Rightarrow>'a \<Rightarrow>'a list \<Rightarrow>'a list" where 
-"update_list _ _ [] =[]"|
-"update_list 0 new_ele (x#xs) =new_ele#xs"|
-"update_list (Suc n) new_ele (x#xs) =x#(update_list n new_ele xs)"
-
-lemma length_update_list:"length ( update_list n a l) =length l"
-  apply (induction  l arbitrary:n a  )
-   apply simp
-  by (smt (verit) length_Cons list.sel(3) update_list.elims)
-
-lemma l1:"k\<ge>1\<and>k\<le>length gs \<longrightarrow>length ((replicate (k - 1) Stay) @ [Left] @ (replicate (length gs - k) Stay)) = length gs"
-  apply simp
-  by auto
-lemma length_replicate:"length ( replicate n a ) =n"
-  by simp
-fun write_bit_tape::"nat \<Rightarrow>nat \<Rightarrow>command" where
-"write_bit_tape b k=( \<lambda> symbols_read_from_tapes.
-      (
-        0, \<comment> \<open>new state\<close>
-        let len =(length symbols_read_from_tapes);
-         new_symbols_of_tapes =(update_list k (b+2) symbols_read_from_tapes);
-        directions = (replicate  (k-1) Stay)@ [Right]@(replicate  (len-k) Stay)
-          in
-       (zip new_symbols_of_tapes  directions)
-      )
-   )"
-
-(*
-definition wf_command :: "nat \<Rightarrow> nat \<Rightarrow> command \<Rightarrow> bool" where
-  "wf_command k Q cmd \<equiv> \<forall>gs. length gs = k \<longrightarrow> length (snd (cmd gs)) = k \<and> fst (cmd gs) \<le> Q"
-*)
-
-
-fun write_end_tape::"nat \<Rightarrow>command" where
-"write_end_tape k=( \<lambda> symbols_read_from_tapes.
-      (
-        1, \<comment> \<open>new state\<close>
-        let len =(length symbols_read_from_tapes);
-         new_symbols_of_tapes =(update_list k 0 symbols_read_from_tapes);
-        directions = (replicate  (k-1) Stay)@ [Left]@(replicate  (len-k) Stay)
-          in
-       (zip new_symbols_of_tapes  directions)
-      )
-   )"
-
-lemma write_end_tape_wf_command:
-  fixes k K Q
-  assumes "k \<ge> 1" and "K \<ge> k" and "Q \<ge> 4"
-  shows "wf_command K Q (write_end_tape k)"
-  using assms
-proof -
-  have x:"wf_command K Q (write_end_tape k) \<longleftrightarrow> (\<forall>gs. length gs = K \<longrightarrow> length (snd (write_end_tape k gs)) = K \<and> fst (write_end_tape k gs) \<le> Q)"
-    by (simp add: wf_command_def)
-  show "wf_command K Q (write_end_tape k)"
-  proof (subst wf_command_def, rule allI, rule impI)
-    fix gs :: "nat list"
-    assume "length gs = K"
-    have "write_end_tape k gs = (
-      let len = length gs;
-          new_symbols_of_tapes = update_list k 0 gs;
-          directions = (replicate (k - 1) Stay) @ [Left] @ (replicate (len - k) Stay)
-      in (2, (zip new_symbols_of_tapes directions))
-    )"
-      by (simp add: write_end_tape.simps)
-    then have cmd_def: "write_end_tape k gs = (
-      let len = length gs;
-          new_symbols_of_tapes = update_list k 0 gs;
-          directions = (replicate (k - 1) Stay) @ [Left] @ (replicate (len - k) Stay)
-      in (2, (zip new_symbols_of_tapes directions))
-    )"
+lemma sem_cmd_minus:
+  assumes "j1 \<noteq> j2"
+    and "j1 < k - 1"
+    and "j2 < k - 1"
+    and "j2 > 0"
+    and "length tps = k"
+    and "bit_symbols xs"
+    and "bit_symbols ys"
+    and "tps ! j1 = (\<lfloor>xs\<rfloor>, Suc t)"
+    and "tps ! j2 = (\<lfloor>map (minusdigit xs ys) [0..<t] @ drop t ys\<rfloor>, Suc t)"
+    and "last tps = \<lceil>carry_minus xs ys t\<rceil>"
+    and "rs = read tps"
+    and "c=carry_minus xs ys (Suc t)"
+    and "tps' = tps
+      [j1 := tps!j1 |+| 1,
+       j2 := tps!j2 |:=| minusdigit xs ys t |+| 1,
+       length tps - 1 := \<lceil>c\<rceil>]"
+  shows "sem (cmd_minus0 j1 j2) (0, tps) = (if t < max (length xs) (length ys) then 0 else if (todigit (last rs) =1) then 1 else 2
+         , tps')"
+proof
+  have "k \<ge> 2"
+    using assms(3,4) by simp
+  have rs1: "rs ! j1 = digit xs t"
+    using assms(2,5,8,11) digit_def read_def contents_def by simp
+  let ?zs = "map (minusdigit xs ys) [0..<t] @ drop t ys"
+  have rs2: "rs ! j2 = digit ys t"
+  proof (cases "t < length ys")
+    case True
+    then have "?zs ! t = ys ! t"
+      by (simp add: nth_append)
+    then show ?thesis
+      using assms(3,5,9,11) digit_def read_def contents_def by simp
+  next
+    case False
+    then have "length ?zs = t"
       by simp
-    (* Check the length of the resulting symbols *)
-    have "length (snd (write_end_tape k gs)) = length (zip (update_list k 0 gs) ((replicate (k - 1) Stay) @ [Left] @ (replicate (length gs - k) Stay)))"
-      by (simp add: cmd_def)
-    moreover have "length (update_list k 0 gs) = length gs"
-    by (simp add: length_update_list)
-    moreover have "length ((replicate (k - 1) Stay) @ [Left] @ (replicate (length gs - k) Stay)) = length gs"
-    using \<open>length gs = K\<close> assms(1) assms(2) l1 by blast
-    ultimately have "length (snd (write_end_tape k gs)) = K"
-      by (simp add: \<open>length gs = K\<close>)
-    (* Check the state *)
-    have "fst (write_end_tape k gs) = 2"
-      by (simp add: cmd_def)
-    then have "fst (write_end_tape k gs) \<le> Q"
-      using \<open>Q \<ge> 4\<close> by simp
-    (* Combine the results *)
-    show "length (snd (write_end_tape k gs)) = K \<and> fst (write_end_tape k gs) \<le> Q"
-    using \<open>[*] write_end_tape k gs \<le> Q\<close> \<open>length ([!!] write_end_tape k gs) = K\<close> by blast
-      (*by (simp add: \<open>length (snd (write_end_tape k gs)) = K\<close> \<open>fst (write_end_tape k gs) \<le> Q\<close>)*)
+    then have "\<lfloor>?zs\<rfloor> (Suc t) = \<box>"
+      using False contents_def by simp
+    then show ?thesis
+      using digit_def read_def contents_def False assms(3,5,9,11) by simp
+  qed
+  have rs3: "last rs = carry_minus xs ys t"
+    using `k \<ge> 2` assms onesie_read onesie_def read_def read_length tapes_at_read'
+    by (metis (no_types, lifting) diff_less last_conv_nth length_greater_0_conv less_one list.size(3) not_numeral_le_zero)
+  have *: "tosym ((todigit (rs ! j1) + todigit (rs ! j2) + todigit (last rs)) mod 2) =  minusdigit xs ys t"
+    using rs1 rs2 rs3 minusdigit_def by simp
+ 
+  have r:"2+ todigit (rs ! j1)> todigit (rs ! j2) - todigit (last rs)" by simp
+  then have  **:"tosym ((2+ todigit (rs ! j1) - todigit (rs ! j2) - todigit (last rs)) mod 2) =minusdigit xs ys t"
+  by (smt (z3) "*" add.commute diff_add_inverse2 minus_nat.diff_0 mod_add_self1 nat_1_add_1)
+
+  have "\<not> (digit xs t = 0 \<and> digit ys t = 0)" if "t < max (length xs) (length ys)"
+    using assms(6,7) digit_def that by auto
+  then have 4: "\<not> (rs ! j1 = 0 \<and> rs ! j2 = 0)" if "t < max (length xs) (length ys)"
+    using rs1 rs2 that by simp
+  then have fst1: "fst (sem (cmd_minus0 j1 j2) (0, tps)) = fst (0, tps')" if "t < max (length xs) (length ys)"
+    using that cmd_minus0_def assms(11) by (smt (verit, ccfv_threshold) fst_conv prod.sel(2) sem)
+
+  have "digit xs t = 0 \<and> digit ys t = 0" if "t \<ge> max (length xs) (length ys)"
+    using that digit_def by simp
+  then have 5: "rs ! j1 = \<box> \<and> rs ! j2 = \<box>" if "t \<ge> max (length xs) (length ys)"
+    using rs1 rs2 that by simp
+  then have q6:"fst (sem (cmd_minus0 j1 j2) (0, tps)) = fst (if todigit(last rs) = 1 then 1 else 2,tps')" if "t \<ge> max (length xs) (length ys)"
+    using that cmd_minus0_def assms(11) by (smt (verit, ccfv_threshold) fst_conv prod.sel(2) sem)
+  then show q7:"fst (sem (cmd_minus0 j1 j2) (0, tps)) = fst (if t < max (length xs) (length ys) then 0 else if (todigit (last rs) =1) then 1 else 2
+         , tps')"
+    using fst1 not_less by fastforce
+  show "snd (sem (cmd_minus0 j1 j2) (0, tps)) = snd (if t < max (length xs) (length ys) then 0 else if (todigit (last rs) =1) then 1 else 2
+         , tps')"
+  proof (rule snd_semI)
+    show "proper_command k (cmd_minus0 j1 j2)"
+      using cmd_minus0_def by simp
+    show "length tps = k"
+      using assms(5) .
+    show "length tps' = k"
+     by (simp add: assms(4,5,13))
+    have len: "length (read tps) = k"
+      by (simp add: assms read_length)
+    show "act (cmd_minus0 j1 j2 (read tps) [!] j) (tps ! j) = tps' ! j"
+      if "j < k" for j
+    proof -
+      have j: "j < length tps"
+        using len that assms(5) by simp
+      consider
+          "j = j1"
+        | "j \<noteq> j1 \<and> j = j2"
+        | "j \<noteq> j1 \<and> j \<noteq> j2 \<and> j = length rs - 1"
+        | "j \<noteq> j1 \<and> j \<noteq> j2 \<and> j \<noteq> length rs - 1"
+        by auto
+      then show ?thesis
+      proof (cases)
+        case 1
+        then have "cmd_minus0 j1 j2 (read tps) [!] j = (read tps ! j, Right)"
+          using that len cmd_minus0_def by simp
+        then have "act (cmd_minus0 j1 j2 (read tps) [!] j) (tps ! j) = tps ! j |+| 1"
+          using act_Right[OF j] by simp
+        moreover have "tps' ! j = tps ! j |+| 1"
+          using assms(1,2,5,6,12,13) that 1 by simp
+        ultimately show ?thesis
+          by force
+      next
+        case 2
+        then have "cmd_minus0 j1 j2 (read tps) [!] j =
+            (tosym ((todigit (rs ! j1) + todigit (rs ! j2) + todigit (last rs)) mod 2), Right)"
+          using that len cmd_minus0_def assms(11) by simp
+        then have "cmd_minus0 j1 j2 (read tps) [!] j = (minusdigit xs ys t, Right)"
+          using * by simp
+        moreover have "tps' ! j2 = tps!j2 |:=| minusdigit xs ys t |+| 1"
+          using assms(3,4,5,6,12,13) by simp
+        ultimately show ?thesis
+          using act_Right' 2 by simp
+      next
+        case 3
+        then have "cmd_minus0 j1 j2 (read tps) [!] j =(if (todigit (rs ! j1) < todigit  (rs ! j2) + todigit (last rs)) then \<one> else \<zero>, Stay)"
+          using that len cmd_minus0_def assms(11) by simp
+        then have "cmd_minus0 j1 j2 (read tps) [!] j = (carry_minus xs ys (Suc t), Stay)"
+          using rs1 rs2 rs3 by simp
+        moreover have "tps' ! (length tps - 1) = \<lceil>c\<rceil>"
+          using 3 assms(5,6,11,12,13) len that by simp
+        ultimately show ?thesis
+          using 3 act_onesie assms(3,4,5,6,10,11,12) len 
+          by (metis add_diff_inverse_nat last_length less_nat_zero_code nat_diff_split_asm plus_1_eq_Suc)
+      next
+        case 4
+        then have "cmd_minus0 j1 j2 (read tps) [!] j = (read tps ! j, Stay)"
+          using that len cmd_minus0_def assms(11) by simp
+        then have "act (cmd_minus0 j1 j2 (read tps) [!] j) (tps ! j) = tps ! j"
+          using act_Stay[OF j] by simp
+        moreover have "tps' ! j = tps ! j"
+          using that 4 len assms(5,6,11,12,13) by simp
+        ultimately show ?thesis
+          by simp
+      qed
+    qed
   qed
 qed
 
-
-
-lemma write_end_tape_wf_command:
-  fixes k K Q
-  assumes "k \<ge> 1" and "K \<ge> k" and "Q \<ge> 4"
-  shows "wf_command K Q (write_end_tape k)"
-  using assms
-  sorry
-
-
-
-fun one_tape_back_start::"nat\<Rightarrow> command" where
-"one_tape_back_start k=( \<lambda> symbols_read_from_tapes.
-      (
-        3, \<comment> \<open>new state\<close>
-        if symbols_read_from_tapes!0 = 0 then 
-        let len =(length symbols_read_from_tapes);
-        directions = (replicate  (k-1) Stay)@ [Right]@(replicate  (len-k) Stay)
-          in
-       (zip symbols_read_from_tapes  directions)
-      else 
-        let len =(length symbols_read_from_tapes);
-        directions = (replicate  (k-1) Stay)@ [Left]@(replicate  (len-k) Stay)
-          in
-       (zip symbols_read_from_tapes  directions)
-      )
-)"
-
-(*
-abbreviation (input) blank_symbol :: nat ("\<box>") where "\<box> \<equiv> 0"
-abbreviation (input) start_symbol :: nat ("\<triangleright>")   where "\<triangleright> \<equiv> 1"
-abbreviation (input) zero_symbol :: nat ("\<zero>")   where "\<zero> \<equiv> 2"
-abbreviation (input) one_symbol :: nat ("\<one>")    where "\<one> \<equiv> 3"
-abbreviation (input) bar_symbol :: nat ("\<bar>")      where "\<bar> \<equiv> 4"
-abbreviation (input) sharp_symbol :: nat ("\<sharp>")  where "\<sharp> \<equiv> 5"
-*)
-
-
-fun write_nat_tape::"nat \<Rightarrow>nat \<Rightarrow> machine" where
-" write_nat_tape 0 k = [write_end_tape k,one_tape_back_start k]"|
-" write_nat_tape n k =  (
-   (write_bit_tape (n mod 2) k)# (write_nat_tape (n div 2 ) k)
-   )"
-
-(*
-definition wf_command :: "nat \<Rightarrow> nat \<Rightarrow> command \<Rightarrow> bool" where
-  "wf_command k Q cmd \<equiv> \<forall>gs. length gs = k \<longrightarrow> length (snd (cmd gs)) = k \<and> fst (cmd gs) \<le> Q"
-*)
-
-
-
-theorem write_nat_maschine:
-  (* there are K tapes in total, and we write a number n to kth tape*)
-  fixes n k K G
-  assumes "k\<ge>1" and "K\<ge>k+1" and "G\<ge>4"
-  shows "turing_machine K G (write_nat_tape n k)  "
-  using assms 
- proof (induction n)
-  case 0
-  then show ?case
-  proof -
-    have "K \<ge> 2" using assms(2) assms(1) by linarith
-    moreover have "G \<ge> 4" using assms(3) by simp
-    moreover have "(\<forall>cmd\<in>set (write_nat_tape 0 k). turing_command K (length (write_nat_tape 0 k)) G cmd)"
-    proof
-      fix cmd
-      assume "cmd \<in> set (write_nat_tape 0 k)"
-      then have "cmd = write_end_tape k \<or> cmd = one_tape_back_start k" 
-        by (simp add: write_nat_tape.simps)
-      then show "turing_command K (length (write_nat_tape 0 k)) G cmd"
-      proof
-        assume "cmd = write_end_tape k"
-        (* Assuming write_end_tape is a valid turing command *)
-        then have "wf_command K G cmd" 
-          by (meson add_leD1 assms(1) assms(2) calculation(2) write_end_tape_wf_command)
-        have "(\<forall>gs. length gs = k \<longrightarrow>
-      ((\<forall>i<k. gs ! i < G) \<longrightarrow> (\<forall>i<k. fst (snd (cmd gs) ! i) < G)) \<and>
-       (k > 0 \<longrightarrow> fst (snd (cmd gs) ! 0) = gs ! 0))"
-        proof -
-           fix gs
-           assume "length gs = k"
-         qed
-      then show "turing_command K (length (write_nat_tape 0 k)) G cmd"
-          by (simp add: turing_command_def wf_command_def) (* 需要假设 write_end_tape 满足 turing_command *)
-      next
-        assume "cmd = one_tape_back_start k"
-        (* Assuming one_tape_back_start is a valid turing command *)
-        then show "turing_command K (length (write_nat_tape 0 k)) G cmd"
-          by (simp add: turing_command_def wf_command_def) (* 需要假设 one_tape_back_start 满足 turing_command *)
-      qed
-    qed
-    ultimately show "turing_machine K G (write_nat_tape 0 k)"
-      by (simp add: turing_machine_def)
-  qed
-next
-  case (Suc n)
-  then show ?case
-  proof -
-    have "K \<ge> 2" using assms(2) by simp
-    moreover have "G \<ge> 4" using assms(3) by simp
-    moreover have "(\<forall>cmd\<in>set (write_nat_tape (Suc n) k). turing_command K (length (write_nat_tape (Suc n) k)) G cmd)"
-    proof
-      fix cmd
-      assume "cmd \<in> set (write_nat_tape (Suc n) k)"
-      then have "cmd = write_bit_tape ((Suc n) mod 2) k \<or> cmd \<in> set (write_nat_tape (Suc n div 2) k)"
-        by (simp add: write_nat_tape.simps)
-      then show "turing_command K (length (write_nat_tape (Suc n) k)) G cmd"
-      proof
-        assume "cmd = write_bit_tape ((Suc n) mod 2) k"
-        (* Assuming write_bit_tape is a valid turing command *)
-        then show "turing_command K (length (write_nat_tape (Suc n) k)) G cmd"
-          by (simp add: turing_command_def wf_command_def) (* 需要假设 write_bit_tape 满足 turing_command *)
-      next
-        assume "cmd \<in> set (write_nat_tape (Suc n div 2) k)"
-        then show "turing_command K (length (write_nat_tape (Suc n) k)) G cmd"
-          using Suc.IH assms(1) assms(2) assms(3) by simp
-      qed
-    qed
-    ultimately show "turing_machine K G (write_nat_tape (Suc n) k)"
-      by (simp add: turing_machine_def)
-  qed
+corollary sem_cmd_minus0':
+  assumes "j1 \<noteq> j2"
+    and "j1 < k - 1"
+    and "j2 < k - 1"
+    and "j2 > 0"
+    and "length tps = k"
+    and "bit_symbols xs"
+    and "bit_symbols ys"
+    and "tps ! j1 = (\<lfloor>xs\<rfloor>, Suc t)"
+    and "tps ! j2 = (\<lfloor>map (minusdigit xs ys) [0..<t] @ drop t ys\<rfloor>, Suc t)"
+    and "last tps = \<lceil>carry_minus xs ys t\<rceil>"
+     and "rs = read tps"
+    and "c=carry_minus xs ys (Suc t)"
+    and "tps' = tps
+      [j1 := (\<lfloor>xs\<rfloor>, Suc (Suc t)),
+       j2 := (\<lfloor>map (minusdigit xs ys) [0..<Suc t] @ drop (Suc t) ys\<rfloor>, Suc (Suc t)),
+       length tps - 1 := \<lceil>c\<rceil>]"
+  shows "sem (cmd_minus0 j1 j2) (0, tps) = (if Suc t \<le> max (length xs) (length ys) then 0 else if (todigit (last rs) =1) then 1 else 2
+         , tps')"
+proof -
+  have "tps ! j1 |+| 1 = (\<lfloor>xs\<rfloor>, Suc (Suc t))"
+    using assms(8) by simp
+  moreover have "tps ! j2 |:=| minusdigit xs ys t |+| 1 =
+      (\<lfloor>map (minusdigit xs ys) [0..<Suc t] @ drop (Suc t) ys\<rfloor>, Suc (Suc t))"
+    using contents_map_append_drop assms(8,9,10,11) by simp
+  ultimately show ?thesis
+    using sem_cmd_minus[OF assms(1-10)] assms(11,12,13) less_eq_Suc_le by presburger
 qed
 
+definition tm_minus :: "tapeidx \<Rightarrow> tapeidx \<Rightarrow> machine" where
+  "tm_minus j1 j2 \<equiv> [cmd_minus0 j1 j2,(cmd_ltrans_until 0 j2 {\<triangleright>} (\<lambda>x. \<box>))]"
 
 
+lemma turing_command_cmd_ltrans_until:"j2 > 0\<longrightarrow>k\<ge>2 \<longrightarrow> G\<ge>4 \<longrightarrow>turing_command k 2 G (cmd_ltrans_until 0 j2 {\<triangleright>} (\<lambda>x. \<box>))"
+  unfolding  cmd_ltrans_until_def using  turing_machine_def by auto
 
-definition stay_direction ::"nat\<Rightarrow>direction list" where
-" stay_direction n=replicate  n Stay"
+lemma tm_plus_tm:
+  assumes "j2 > 0" and "k \<ge> 2" and "G \<ge> 4"
+  shows "turing_machine k G (tm_minus j1 j2)"
+  unfolding tm_minus_def cmd_ltrans_until_def using assms(1-3) cmd_minus0_def turing_machine_def  turing_command_cmd_ltrans_until
+  by auto
 
-definition two_tapes_move_right :: "nat \<Rightarrow>nat\<Rightarrow>nat\<Rightarrow>direction list" where
-  "two_tapes_move_right k1 k2 n=(update_list k1 Right(update_list k2 Right (stay_direction n)))"
-
-definition two_tapes_move_left :: "nat \<Rightarrow>nat\<Rightarrow>nat\<Rightarrow>direction list" where
-  "two_tapes_move_left k1 k2 n=(update_list k1 Left(update_list k2 Left (stay_direction n)))"
-
- \<comment> \<open>copy k2 to k1\<close>
-fun copy_tape::" nat\<Rightarrow>nat \<Rightarrow>command" where
-"copy_tape k1 k2 =(\<lambda> symbols_read_from_tapes.
-      (
-       if symbols_read_from_tapes!k2 = 0 then 5 else 4
-        , \<comment> \<open>new state\<close>
-        if symbols_read_from_tapes!k2 = 0 then 
-        let 
-          len =(length symbols_read_from_tapes);
-          new_symbol_tape=(update_list k1 0 symbols_read_from_tapes);
-          directions =(two_tapes_move_left k1 k2 len)
-          in
-       (zip symbols_read_from_tapes  directions)
-      else 
-        let 
-            len =(length symbols_read_from_tapes);
-           new_symbol_tape=(update_list k1 (symbols_read_from_tapes!k2) symbols_read_from_tapes);
-        directions = (two_tapes_move_right k1 k2 len)
-          in
-       (zip symbols_read_from_tapes  directions)
-      )
-)"
-
-fun two_tape_back_start::"nat\<Rightarrow>nat\<Rightarrow> command" where
-"two_tape_back_start k1 k2=( \<lambda> symbols_read_from_tapes.
-      (
-        6, \<comment> \<open>new state\<close>
-        if symbols_read_from_tapes!0 = 0 then 
-        let len =(length symbols_read_from_tapes);
-        directions = (two_tapes_move_right k1 k2 len)
-          in
-       (zip symbols_read_from_tapes  directions)
-      else 
-        let 
-        len =(length symbols_read_from_tapes);
-        directions =(two_tapes_move_left k1 k2 len)
-          in
-       (zip symbols_read_from_tapes  directions)
-      )
-)"
-
-(*TODO *)
-fun add_two_tape::"nat\<Rightarrow>nat\<Rightarrow>command"  where
-"add_two_tape k1 k2=(\<lambda>l. (0,[])) "
-
-(*TODO *)
-fun sub_two_tape::"nat\<Rightarrow>nat\<Rightarrow>command"  where
-"sub_two_tape k1 k2=(\<lambda>l. (0,[])) "
+lemma tm_minus_immobile:
+  fixes k :: nat
+  assumes "j1 < k" and "j2 < k"
+  shows "immobile (tm_minus j1 j2) k (Suc k)"
+proof -
+  let ?M = "tm_minus j1 j2"
+  { fix q :: nat and rs :: "symbol list"
+    assume q: "q < length ?M"
+    assume rs: "length rs = Suc k"
+    then have len: "length rs - 1 = k"
+      by simp
+    have neq: "k \<noteq> j1" "k \<noteq> j2"
+      using assms by simp_all
+    have M_0:"?M ! 0 = cmd_minus0 j1 j2"
+      using tm_minus_def q by simp
+     have M_1:"?M ! 1= (cmd_ltrans_until 0 j2 {\<triangleright>} (\<lambda>x. \<box>))"
+       using tm_minus_def q by auto
+     have "(cmd_ltrans_until 0 j2 {\<triangleright>} (\<lambda>x. \<box>)) rs [!] k =
+        (rs!k,Stay)"
+       unfolding  cmd_ltrans_until_def using cmd_ltrans_until_def rs len neq 
+       by (smt (verit) add_0 assms(2) diff_zero length_upt lessI less_nat_zero_code nth_map nth_upt snd_conv)
+     have "(cmd_ltrans_until 0 j2 {\<triangleright>} (\<lambda>x. \<box>)) rs [!] k =
+        (rs!k,Stay)"
+       unfolding  cmd_ltrans_until_def using cmd_ltrans_until_def rs len neq 
+     by (smt (verit) add_0 assms(2) diff_zero length_upt lessI less_nat_zero_code nth_map nth_upt snd_conv)
+     then have ee:"(cmd_ltrans_until 0 j2 {\<triangleright>} (\<lambda>x. \<box>)) rs [~] k =
+        Stay" by auto
+  
+   moreover have "(cmd_minus0 j1 j2) rs [!] k =
+        (tosym (if todigit (rs ! j1) < todigit (rs ! j2) + todigit (last rs) then 1 else 0), Stay)"
+      using cmd_minus0_def rs len neq by fastforce
+    then have "(cmd_minus0 j1 j2) rs [~] k = Stay\<and> (cmd_ltrans_until 0 j2 {\<triangleright>} (\<lambda>x. \<box>)) rs [~] k =
+        Stay" using ee by simp
+    then  have "((tm_minus j1 j2)!0) rs [~] k = Stay\<and> ((tm_minus j1 j2)!1) rs [~] k = Stay" using M_0 M_1 by simp
+    moreover have "length (tm_minus j1 j2)=2"unfolding tm_minus_def by auto
+    ultimately have "\<forall>l<length (tm_minus j1 j2). ((tm_minus j1 j2)!l) rs [~] k = Stay" 
+    using One_nat_def less_2_cases_iff by presburger
+  }
+  then show ?thesis unfolding immobile_def by blast
+qed
 
 (*
-datatype aexp =  A atomExp            |
-                 Plus atomExp atomExp |
-                 Sub atomExp atomExp  | 
-                 Parity atomExp       |
-                 RightShift atomExp
+fun count_atomExp_variable ::"atomExp \<Rightarrow>vname set" where
+"count_atomExp_variable (N val) ={}"| 
+"count_atomExp_variable (V vname) ={vname}"
+
+fun count_aexp_variable::"aexp \<Rightarrow>vname set" where
+"count_aexp_variable (A a) =count_atomExp_variable a "|
+"count_aexp_variable  (Plus a b)=(count_atomExp_variable a)\<union>(count_atomExp_variable b)" |
+"count_aexp_variable  (Sub a b)=(count_atomExp_variable a)\<union>(count_atomExp_variable b)" |
+"count_aexp_variable (Parity a) =count_atomExp_variable a "|
+"count_aexp_variable  (RightShift a) =count_atomExp_variable a "              
+
+fun count_com_variable::"com \<Rightarrow>vname set" where
+"count_com_variable  SKIP ={}"|
+"count_com_variable (Assign vname a) ={vname}\<union> (count_aexp_variable a)"|
+"count_com_variable (Seq Seq1 Seq2)=(count_com_variable Seq1)\<union> (count_com_variable Seq2)"|
+"count_com_variable (If vname com1 com2) = {vname}\<union> (count_com_variable com1)\<union> (count_com_variable com2)"|
+"count_com_variable (While  vname com1) = {vname}\<union> (count_com_variable com1)"
+
+(*TODO : numbering every variable from 1*) 
+fun num_variable::" com \<Rightarrow> (vname \<Rightarrow> nat)" where
+"num_variable com  =(\<lambda>s. 1)"
+
 *)
+(* TODO *)    
 
 fun atomExp_TM::"(vname\<Rightarrow>nat) \<Rightarrow>atomExp \<Rightarrow> nat \<Rightarrow>machine" where
-"atomExp_TM idd (N a) s =(write_nat_tape a s)"|
-"atomExp_TM idd (V v) s =[copy_tape (idd v) s]"
+"atomExp_TM idd (N a) tp =[]"|
+"atomExp_TM idd (V v) tp =tm_cp_until (idd v) tp {\<box>}"
 
-
-(* TODO *)
-
-fun Aexp_TM::"(vname\<Rightarrow>nat)\<Rightarrow>aexp \<Rightarrow>machine " where
-"Aexp_TM idd (A a ) = atomExp_TM idd a 1"|
-"Aexp_TM idd (Plus a1 a2) = (atomExp_TM idd a1 1);;( atomExp_TM idd a2 2);;[add_two_tape 1 2]"|
-"Aexp_TM idd (Sub a1 a2) = (atomExp_TM idd a1 1);; (atomExp_TM idd a2 2);;[sub_two_tape 1 2]"|
-"Aexp_TM idd (Parity a) = []"|
-"Aexp_TM idd (RightShift a) = []"
+fun Aexp_TM::"(vname\<Rightarrow>nat)\<Rightarrow>aexp \<Rightarrow> machine " where
+"Aexp_TM idd (A a ) = ( atomExp_TM idd a 2)"|
+"Aexp_TM idd (Plus a1 a2) = (atomExp_TM idd a1 1) ;; ( atomExp_TM idd a2 2);;tm_plus 1 2"|
+"Aexp_TM idd (Sub a1 a2) = (atomExp_TM idd a1 1);;(atomExp_TM idd a2 2);;tm_minus 1 2"|
+"Aexp_TM idd (Parity a) = (atomExp_TM idd a 2);;(tm_mod2 2 2)"|
+"Aexp_TM idd (RightShift a) =(atomExp_TM idd a 2);;(tm_div2 2)"
 
 (*
 TODO:read value from a tape
 *)
+
 fun tape_list_read::"nat \<Rightarrow>nat" where
 " tape_list_read k = 0"
-
 (*
-datatype
-  com = SKIP 
-      | Assign vname aexp      
-      | Seq    com  com         
-      | If     vname com com     
-      | While  vname com
-*)
-(* IF cond THEN M1 ELSE M2 ENDIF*)
-(*(symbol list \<Rightarrow> bool)*)
-
-
-(*
-text \<open>
-The loops are while loops consisting of a head and a body. The body is a Turing
-machine that is executed in every iteration as long as the condition in the
-head of the loop evaluates to true. The condition is of the same form as in
-branching TMs, namely a predicate over the symbols read from the tapes.
-Sometimes this is not expressive enough, and so we allow a Turing machine as
-part of the loop head that is run prior to evaluating the condition. In most
-cases, however, this TM is empty.
-\<close>
-
-definition turing_machine_loop :: "machine \<Rightarrow> (symbol list \<Rightarrow> bool) \<Rightarrow> machine \<Rightarrow> machine"
-  ("WHILE _ ; _ DO _ DONE" 60)
-where
-  "WHILE M1 ; cond DO M2 DONE \<equiv>
-    M1 @
-    [cmd_jump cond (length M1 + 1) (length M1 + length M2 + 2)] @
-    (relocate (length M1 + 1) M2) @
-    [cmd_jump (\<lambda>_. True) 0 0]"
-*)
-
-(*
-definition turing_machine_branch :: "(symbol list \<Rightarrow> bool) \<Rightarrow> machine \<Rightarrow> machine \<Rightarrow> machine"
-  ("IF _ THEN _ ELSE _ ENDIF" 60)
-where
-  "IF cond THEN M1 ELSE M2 ENDIF \<equiv>
-    [cmd_jump cond 1 (length M1 + 2)] @
-    (relocate 1 M1) @
-    [cmd_jump (\<lambda>_. True) (length M1 + length M2 + 2) 0] @
-    (relocate (length M1 + 2) M2)"
-*)
-
-(* TODO: cond*)
-
-(* ? ? ? *)
-
 fun while_TM_aux::" com\<Rightarrow>(vname\<Rightarrow>nat) \<Rightarrow>nat \<Rightarrow> machine" where
 "while_TM_aux   SKIP idd k  = []"|
-"while_TM_aux  (Assign v a) idd k  = (Aexp_TM idd a);;[copy_tape 1 (idd v)] "|
-"while_TM_aux  (Seq c1 c2) idd k = (while_TM_aux c1 idd k);;(while_TM_aux c2 idd k)"|
-"while_TM_aux  (If v c1 c2) idd k =IF (\<lambda>x. True) THEN (while_TM_aux c1 idd k) ELSE (while_TM_aux c1 idd k) ENDIF"|
-"while_TM_aux  (While  v c) idd k = (while_TM_aux  (If v c SKIP) idd k);;while_TM_aux  (While  v c) idd k"
-
-
-
-definition while_TM ::"com \<Rightarrow>machine" where
-"while_TM c =while_TM_aux c (num_variable c) (card(count_com_variable c)+3)"
-
-
-
-theorem while_TM_is_Turing:"turing_machine 5 (card(count_com_variable c)) (while_TM c)"
-  sorry
-
-(* the first tape is not needed, so I will let it be empty for the sake of convenience*)
-(*definition start_config :: "nat \<Rightarrow> symbol list \<Rightarrow> config" where
-  "start_config k xs \<equiv> (0, (\<lfloor>xs\<rfloor>, 0) # replicate (k - 1) (\<lfloor>[]\<rfloor>, 0))"
+"while_TM_aux  (Assign v a) idd k  =  ((Aexp_TM idd a);;(tm_cp_until 2 (idd v) {\<box>}))"|
+"while_TM_aux  (Seq c1 c2) idd k = ((while_TM_aux c1 idd k);;(while_TM_aux c2 idd k))"|
+"while_TM_aux  (If v c1 c2) idd k =((tm_cmp 0 (idd v) 2);; IF (\<lambda>x. x!2=0) THEN (while_TM_aux c1 idd k) ELSE (while_TM_aux c1 idd k) ENDIF)"|
+"while_TM_aux  (While  v c) idd k =(WHILE (tm_cmp 0 (idd v) 2) ; (\<lambda>x. x!2=0) DO while_TM_aux c idd k DONE)"
 *)
-abbreviation cfg0 ::"com \<Rightarrow>config" where
-"cfg0 c \<equiv> start_config (card(count_com_variable c)) []"
+
+fun while_TM_aux::" com\<Rightarrow> (vname\<Rightarrow>nat) \<Rightarrow> machine" where
+"while_TM_aux   SKIP idd   = []"|
+"while_TM_aux  (Assign v a) idd  =  ((Aexp_TM idd a);;(tm_cp_until 2 (idd v) {\<box>}))"|
+"while_TM_aux  (Seq c1 c2) idd = ((while_TM_aux c1 idd);;(while_TM_aux c2 idd))"|
+"while_TM_aux  (If v c1 c2) idd =((tm_cmp 0 (idd v) 2);; IF (\<lambda>x. x!2=0) THEN (while_TM_aux c1 idd) ELSE (while_TM_aux c1 idd) ENDIF)"|
+"while_TM_aux  (While  v c) idd =(WHILE (tm_cmp 0 (idd v) 2) ; (\<lambda>x. x!2=0) DO while_TM_aux c idd DONE)"
 
 
-theorem while_TM_halts :
-  assumes "\<exists>n. (c,(\<lambda>x. 0)) \<Rightarrow>\<^bsup> n \<^esup> t"
-  shows " halts (while_TM c) (cfg0 c) "
+inductive
+  big_step_Logt :: "com \<times> AExp.state \<Rightarrow> nat \<Rightarrow> AExp.state \<Rightarrow> bool"  ("_ \<Rightarrow>\<^bsup> _ \<^esup>\<^esup> _" 55)
+where
+Skip: "(SKIP,s) \<Rightarrow>\<^bsup> Suc (0::nat) \<^esup>\<^esup> s"|
+Assign_vname: "(x ::= a, s) \<Rightarrow>\<^bsup> Suc (nlength (aval a s)) \<^esup>\<^esup> s(x := aval a s)" |
+Seq: "\<lbrakk> (c1,s1) \<Rightarrow>\<^bsup> x \<^esup>\<^esup> s2;  (c2,s2) \<Rightarrow>\<^bsup> y \<^esup>\<^esup> s3 ;z=x+y\<rbrakk> \<Longrightarrow> (c1;;c2, s1) \<Rightarrow>\<^bsup>z \<^esup>\<^esup> s3" |
+IfTrue: "\<lbrakk> s b \<noteq> 0;  (c1,s) \<Rightarrow>\<^bsup> x \<^esup>\<^esup> t; y=x+1 \<rbrakk> \<Longrightarrow> (IF b \<noteq>0 THEN c1 ELSE c2, s) \<Rightarrow>\<^bsup> y \<^esup>\<^esup> t" |
+IfFalse: "\<lbrakk> s b = 0; (c2,s) \<Rightarrow>\<^bsup> x \<^esup>\<^esup> t; y=x+1  \<rbrakk> \<Longrightarrow> (IF b \<noteq>0 THEN c1 ELSE c2, s) \<Rightarrow>\<^bsup> y \<^esup>\<^esup> t" |
+WhileFalse: "\<lbrakk> s b = 0 \<rbrakk> \<Longrightarrow> (WHILE b \<noteq>0 DO c,s) \<Rightarrow>\<^bsup> Suc (Suc 0)\<^esup>\<^esup> s" |
+WhileTrue: "\<lbrakk> s1 b \<noteq> 0;  (c,s1) \<Rightarrow>\<^bsup> x\<^esup>\<^esup> s2;  (WHILE b \<noteq>0 DO c, s2) \<Rightarrow>\<^bsup> y \<^esup>\<^esup> s3; 1+x+y=z  \<rbrakk> 
+    \<Longrightarrow> (WHILE b \<noteq>0 DO c, s1) \<Rightarrow>\<^bsup> z \<^esup>\<^esup> s3" 
 
+
+
+declare big_step_Logt.intros [intro]
+
+text "Induction rules with pair splitting"
+lemmas big_step_Logt_induct = big_step_Logt.induct[split_format(complete)]
+
+subsection "Rule inversion"
+inductive_cases Skip_tE[elim!]: "(SKIP,s) \<Rightarrow>\<^bsup> x \<^esup>\<^esup> t"
+inductive_cases Assign_tE[elim!]: "(x ::= a,s) \<Rightarrow>\<^bsup> p  \<^esup>\<^esup> t"
+inductive_cases Seq_tE[elim!]: "(c1;;c2,s1) \<Rightarrow>\<^bsup> p \<^esup>\<^esup> s3"
+inductive_cases If_tE[elim!]: "(IF b \<noteq>0 THEN c1 ELSE c2,s) \<Rightarrow>\<^bsup> x  \<^esup>\<^esup>  t"
+inductive_cases While_tE[elim]: "(WHILE b \<noteq>0 DO c,s) \<Rightarrow>\<^bsup> x  \<^esup>\<^esup>  t"
+lemma Seq': "\<lbrakk> (c1,s1) \<Rightarrow>\<^bsup> x  \<^esup>\<^esup>  s2;  (c2,s2) \<Rightarrow>\<^bsup> y  \<^esup>\<^esup>  s3  \<rbrakk> \<Longrightarrow> (c1;;c2, s1) \<Rightarrow>\<^bsup> x + y  \<^esup>\<^esup>  s3"
+  by auto
+
+text "Rule inversion use examples:"
+lemma "(IF b \<noteq>0 THEN SKIP ELSE SKIP, s) \<Rightarrow>\<^bsup> x  \<^esup>\<^esup>  t \<Longrightarrow> t = s"
+  by blast
+
+lemma assumes "(IF b \<noteq>0 THEN SKIP ELSE SKIP, s) \<Rightarrow>\<^bsup> x  \<^esup>\<^esup>  t"
+  shows "t = s"
+  using assms apply cases by auto
+
+lemma assign_t_simp:
+  "((x ::= a,s) \<Rightarrow>\<^bsup>Suc (nlength (aval a s))\<^esup>\<^esup>   s') \<longleftrightarrow> (s' = s(x := aval a s))"
+  by (auto)
+
+subsection "Determinism of Big semantics of IMP-"
+theorem big_step_t_determ2: "\<lbrakk> (c,s) \<Rightarrow>\<^bsup> p \<^esup>\<^esup> t; (c,s) \<Rightarrow>\<^bsup> q \<^esup>\<^esup> u \<rbrakk> \<Longrightarrow> (u = t \<and> p=q)"
+  apply  (induction arbitrary: u q rule: big_step_Logt_induct)
+    apply(elim Skip_tE) apply(simp)
+    apply(elim Assign_tE) apply(simp)
+  apply blast
+    apply(elim If_tE) apply(simp) apply blast
+    apply(elim If_tE)  apply (linarith) apply simp
+    apply(erule While_tE) apply(simp) apply simp
+  subgoal premises p for s1 b c x s2 y s3 z u q
+    using p(7) apply(safe) 
+      apply(erule While_tE)
+        using p(1-6) apply fast
+        using p(1-6) apply (simp)
+      apply(erule While_tE)
+        using p(1-6) apply fast
+        using p(1-6) by (simp)
+done
+
+lemma bigstep_det: "(c1, s) \<Rightarrow>\<^bsup> p1\<^esup>\<^esup>t1 \<Longrightarrow> (c1, s) \<Rightarrow>\<^bsup> p \<^esup>\<^esup> t \<Longrightarrow> p1=p \<and> t1=t"
+  using big_step_t_determ2 by simp
+
+
+lemma seq_is_noop[simp]: "(SKIP, s) \<Rightarrow>\<^bsup>t\<^esup>\<^esup> s' \<longleftrightarrow> (t = Suc 0 \<and> s = s')" by auto
+
+lemma seq_skip[simp]: "(c ;; SKIP, s) \<Rightarrow>\<^bsup>Suc t\<^esup>\<^esup> s' \<longleftrightarrow> (c, s) \<Rightarrow>\<^bsup>t\<^esup>\<^esup> s'" by auto
+
+subsection "Progress property"
+text "every command costs time"
+lemma bigstep_progress: "(c, s) \<Rightarrow>\<^bsup> p \<^esup>\<^esup> t \<Longrightarrow> p > 0"
+  apply(induct rule: big_step_Logt.induct, auto) done
+
+
+
+lemma terminates_in_state_intro: "(c, s) \<Rightarrow>\<^bsup>t \<^esup>\<^esup> s' \<Longrightarrow> s' = s'' \<Longrightarrow> (c, s) \<Rightarrow>\<^bsup>t \<^esup>\<^esup> s''"
+  by simp
+
+lemma terminates_in_time_state_intro: "(c, s) \<Rightarrow>\<^bsup>t \<^esup>\<^esup> s' \<Longrightarrow> t = t' \<Longrightarrow> s' = s'' 
+  \<Longrightarrow> (c, s) \<Rightarrow>\<^bsup>t' \<^esup>\<^esup> s''"
+  by simp
+
+lemma terminates_in_time_state_intro': "(c', s) \<Rightarrow>\<^bsup>t \<^esup>\<^esup> s' \<Longrightarrow> t = t' \<Longrightarrow> s' = s'' \<Longrightarrow> c' = c
+  \<Longrightarrow> (c, s) \<Rightarrow>\<^bsup>t' \<^esup>\<^esup> s''"
+  by simp
+
+method dest_com  = 
+  (match premises in a: "\<lbrakk>loop_cond; state_upd\<rbrakk> \<Longrightarrow> (_, s) \<Rightarrow>\<^bsup>t \<^esup>\<^esup> s'"
+    for s s' t loop_cond state_upd \<Rightarrow> \<open>rule terminates_in_time_state_intro'[OF a]\<close>)
+
+method dest_com' = 
+  (match premises in a[thin]: "\<lbrakk>loop_cond; state_upd; (_, s) \<Rightarrow>\<^bsup>t \<^esup>\<^esup>s'\<rbrakk> \<Longrightarrow> P" 
+    for s s' t loop_cond state_upd P  \<Rightarrow>
+   \<open>match premises in b[thin]: "(While _ _, s2) \<Rightarrow>\<^bsup>t2 \<^esup>\<^esup>s2'"
+      for s2 s2' t2 \<Rightarrow> \<open>insert a[OF _ _ b]\<close>\<close>)
+
+
+method dest_com_init_while = 
+  (match premises in a[thin]: "\<lbrakk>loop_cond; state_upd; ((_ ;; While _ _), s) \<Rightarrow>\<^bsup>t \<^esup>\<^esup> s'\<rbrakk> \<Longrightarrow> P" 
+    for s s' t loop_cond state_upd P  \<Rightarrow>
+   \<open>match premises in b[thin]: "((_ ;; While _ _), s2) \<Rightarrow>\<^bsup>t2 \<^esup>\<^esup> s2'"
+      for s2 s2' t2 \<Rightarrow> \<open>insert a[OF _ _ b]\<close>\<close>)
+
+
+
+lemma terminates_split_if : "(P s \<Longrightarrow> (c, s) \<Rightarrow>\<^bsup>t1 \<^esup>\<^esup> s1 ) \<Longrightarrow> 
+(\<not> P s \<Longrightarrow> (c, s) \<Rightarrow>\<^bsup>t2 \<^esup>\<^esup>s2 ) \<Longrightarrow> (c,s) \<Rightarrow>\<^bsup>if P s then t1 else t2 \<^esup>\<^esup>  if P s then s1 else s2"
+  by auto
+
+lemma AssignD': 
+"(x ::= a, s) \<Rightarrow>\<^bsup> 2\<^esup>\<^esup> s' \<Longrightarrow> s' = s (x:= aval a s)"
+  by (auto simp add: eval_nat_numeral)
+
+lemma com_only_vars: "\<lbrakk>(c, s) \<Rightarrow>\<^bsup> t  \<^esup>\<^esup> s'; x \<notin> set (Max_Constant.all_variables c)\<rbrakk> \<Longrightarrow> s x = s' x"
+  by (induction arbitrary: t rule: big_step_Logt_induct)  auto
+
+lemma Seq'': "\<lbrakk> (c1,s1) \<Rightarrow>\<^bsup> x  \<^esup>\<^esup> s2 \<and> P s2; P s2 \<Longrightarrow> (c2,s2) \<Rightarrow>\<^bsup> y  \<^esup>\<^esup> s3 \<and> Q s3; Q s3 \<Longrightarrow> R s3 \<rbrakk>
+             \<Longrightarrow> (c1;;c2, s1) \<Rightarrow>\<^bsup> x + y  \<^esup>\<^esup> s3 \<and> R s3"
+  by auto
+
+lemma WhileI:
+"\<lbrakk>(s1 b \<noteq> 0 \<Longrightarrow> (c,s1) \<Rightarrow>\<^bsup> x  \<^esup>\<^esup> s2 \<and> (WHILE b \<noteq>0 DO c, s2) \<Rightarrow>\<^bsup> y  \<^esup>\<^esup> s3);
+  (s1 b = 0 \<Longrightarrow> s1 = s3);
+  z = (if s1 b \<noteq> 0 then 1+x+y else 2)\<rbrakk>
+        \<Longrightarrow> (WHILE b \<noteq>0 DO c, s1) \<Rightarrow>\<^bsup> z  \<^esup>\<^esup> s3" 
+  by (auto simp add: WhileTrue WhileFalse numeral_2_eq_2)
+
+lemma IfI:
+"\<lbrakk>s b \<noteq> 0 \<Longrightarrow> (c1,s) \<Rightarrow>\<^bsup> x1  \<^esup>\<^esup> t1;
+  s b = 0 \<Longrightarrow> (c2,s) \<Rightarrow>\<^bsup> x2  \<^esup>\<^esup> t2;
+  y = (if s b \<noteq> 0 then x1 else x2) + 1;
+  t = (if s b \<noteq> 0 then t1 else t2)\<rbrakk>
+        \<Longrightarrow> (IF b \<noteq>0 THEN c1 ELSE c2, s) \<Rightarrow>\<^bsup> y  \<^esup>\<^esup> t" 
+  by (auto simp add: IfTrue IfFalse)
+
+lemma IfE: 
+"(IF b \<noteq>0 THEN c1 ELSE c2, s) \<Rightarrow>\<^bsup> (if s b \<noteq> 0 then x1 else x2) + 1  \<^esup>\<^esup> (if s b \<noteq> 0 then s1 else s2) \<Longrightarrow> 
+ \<lbrakk>\<lbrakk>s b \<noteq> 0; (if s b \<noteq> 0 then x1 else x2) + 1 = x1 + 1; 
+  (if s b \<noteq> 0 then s1 else s2) = s1; (c1,s) \<Rightarrow>\<^bsup> x1  \<^esup>\<^esup> s1\<rbrakk> \<Longrightarrow> P;
+  \<lbrakk>s b = 0; (if s b \<noteq> 0 then x1 else x2) + 1 = x2 + 1;
+   (if s b \<noteq> 0 then s1 else s2) = s2; (c2,s) \<Rightarrow>\<^bsup> x2  \<^esup>\<^esup>s2\<rbrakk> \<Longrightarrow> P\<rbrakk>
+        \<Longrightarrow> P"
+  by (auto simp add: IfTrue IfFalse)
+
+thm Seq_tE
+
+lemma IfD:
+"(IF b \<noteq>0 THEN c1 ELSE c2, s) \<Rightarrow>\<^bsup> (if s b \<noteq> 0 then x1 else x2) + 1  \<^esup>\<^esup> (if s b \<noteq> 0 then t1 else t2) \<Longrightarrow> 
+ \<lbrakk>\<lbrakk>s b \<noteq> 0; (c1,s) \<Rightarrow>\<^bsup> x1  \<^esup>\<^esup> t1\<rbrakk> \<Longrightarrow> P;
+  \<lbrakk>s b = 0; (c2,s) \<Rightarrow>\<^bsup> x2  \<^esup>\<^esup> t2\<rbrakk> \<Longrightarrow> P\<rbrakk>
+        \<Longrightarrow> P" 
+  by (auto simp add: IfTrue IfFalse)
+
+
+
+
+lemma AssignI:
+"\<lbrakk>s' = s (x:= aval a s)\<rbrakk>
+        \<Longrightarrow> (x ::= a, s) \<Rightarrow>\<^bsup> Suc (nlength (aval a s))  \<^esup>\<^esup> s'" 
+  by (auto simp add: Assign)
+
+
+lemma AssignD: "(x ::= a, s) \<Rightarrow>\<^bsup> t  \<^esup>\<^esup> s' \<Longrightarrow> t = Suc (nlength (aval a s)) \<and> s' = s(x := aval a s)"
+  by auto
+
+lemma compose_programs_1:
+  "(c2, s2) \<Rightarrow>\<^bsup> y  \<^esup>\<^esup>s3 \<Longrightarrow> (c1, s1) \<Rightarrow>\<^bsup> x \<^esup>\<^esup> s2 \<Longrightarrow> 
+    ((c1;; c2, s1) \<Rightarrow>\<^bsup> x + y  \<^esup>\<^esup>s3 \<Longrightarrow> P)
+   \<Longrightarrow> P"
+  by auto
+
+lemma compose_programs_2:
+  "(c1, s1) \<Rightarrow>\<^bsup> x  \<^esup>\<^esup> s2 \<Longrightarrow> (c2, s2) \<Rightarrow>\<^bsup> y  \<^esup>\<^esup> s3 \<Longrightarrow> 
+    ((c1;; c2, s1) \<Rightarrow>\<^bsup> x + y  \<^esup>\<^esup> s3 \<Longrightarrow> P)
+   \<Longrightarrow> P"
+  by auto
+
+lemma While_tE_time:
+"(WHILE b\<noteq>0 DO c, s) \<Rightarrow>\<^bsup> x  \<^esup>\<^esup> t \<Longrightarrow>
+  (x = Suc (Suc 0) \<Longrightarrow> t = s \<Longrightarrow> s b = 0 \<Longrightarrow> P) \<Longrightarrow>
+  (\<And>x' s2 y. 0 < s b \<Longrightarrow> (c, s) \<Rightarrow>\<^bsup> x'  \<^esup>\<^esup> s2 \<Longrightarrow> (WHILE b\<noteq>0 DO c, s2) \<Rightarrow>\<^bsup> y  \<^esup>\<^esup> t \<Longrightarrow> x = Suc (x' + y) \<Longrightarrow> P) \<Longrightarrow> P"
+  by auto
+
+lemma Seq_tE_While_init:
+  "(WHILE v \<noteq>0 DO c2, s2) \<Rightarrow>\<^bsup> y  \<^esup>\<^esup> s3 \<Longrightarrow> (c1, s1) \<Rightarrow>\<^bsup> x  \<^esup>\<^esup> s2 \<Longrightarrow> 
+    ((c1;; WHILE v \<noteq>0 DO c2, s1) \<Rightarrow>\<^bsup> x + y  \<^esup>\<^esup> s3 \<Longrightarrow> P)
+   \<Longrightarrow> P"
+  by auto
+
+
+abbreviation TP0::"com\<Rightarrow>tape list" where
+"TP0 prog\<equiv> IMPminus_state_to_TM_tape_list prog (\<lambda>x.(0::nat))"
+
+
+(*
+An appropriate idd must satisfies the following condition:
+(1) \forall x \in var_set prog, idd x \<ge>3 
+\<and> Max(idd`(var_set prog))<last_tape 
+*)
+
+lemma length_tps_stable:
+  assumes"transforms M tps1 t tps2"
+  shows"length tps1=length tps2"
   sorry
 
+lemma ineq4:" (a+b::nat)^4\<ge>a^4+b^4"
+  sorry
 
-(* transforms_turing_machine_sequential *)
-(* 
+lemma 
+  fixes t::"nat"
+  and prog::"com"
+  and M::"machine"
+  and idd::"vname\<Rightarrow>nat"
+  and s::"AExp.state"
+  and s'::"AExp.state"
+  and tps::"tape list"
+ assumes asm1:"M = while_TM_aux prog idd"
+ and asm2:"(prog, s)\<Rightarrow>\<^bsup>t\<^esup>\<^esup>s'"                
+ and asm3:"inj idd \<and> (\<forall>x\<in>(var_set prog). (idd x) \<ge>3) "
+ and asm4:"prog (idd) \<turnstile> tps \<sim> s "
+shows "\<exists>tps'. transforms M tps ((100::nat) * t ^ 4) tps'\<and>
+       prog (idd) \<turnstile> tps' \<sim> s'"
+
+(*
+proof-
+  have "(a + b :: nat)^4 = (\<Sum>k\<le>4. (of_nat (4 choose k)) * a^k * b^(4 - k))"  using binomial by blast
+  have "...= a^4+((\<Sum>k\<le>3. (of_nat (4 choose k)) * a^k * b^(4 - k)))"  
+    by (simp add: add.commute binomial_n_n numeral_1_eq_Suc_0 numeral_Bit0 numeral_Bit1 numeral_One of_nat_Suc of_nat_id sum.atMost_Suc)
+  have "k\<le>3\<longrightarrow>a^k*b^(4-k)\<ge>0"by simp
+  then have "(\<Sum>k\<le>3. (of_nat (4 choose k)) * a^k * b^(4 - k))\<ge>(\<Sum>k\<le>1. (of_nat (4 choose k)) * a^k * b^(4 - k))" by sledgehammer
+*)
+theorem lemma_IMPminus_to_TM_correct:
+  fixes t::"nat"
+  and prog::"com"
+  and M::"machine"
+  and idd::"vname\<Rightarrow>nat"
+  and s::"AExp.state"
+  and s'::"AExp.state"
+  and tps::"tape list"
+ assumes asm1:"M = while_TM_aux prog idd"
+ and asm2:"(prog, s)\<Rightarrow>\<^bsup>t\<^esup>\<^esup>s'"                
+ and asm3:"inj idd \<and> (\<forall>x\<in>(var_set prog). (idd x) \<ge>3) "
+ and asm4:"prog (idd) \<turnstile> tps \<sim> s "
+shows "\<exists>tps'. transforms M tps ((100::nat) * t ^ 4) tps'\<and>
+       prog (idd) \<turnstile> tps' \<sim> s'"
+using assms
+proof(induction prog arbitrary:s s' t M tps)
+  case SKIP
+  have "s=s'\<and> t=1" using bigstep_det using SKIP.prems(2) by auto
+  have "M = []" using while_TM_aux.simps(1) by (simp add: SKIP.prems(1))
+  then have "transforms M tps 0 tps" using transforms_Nil by auto
+  then have "transforms M tps ((100::nat) * t ^ 4) tps" using transforms_monotone by blast
+  moreover have " SKIP (idd) \<turnstile> tps \<sim> s" using SKIP.prems(4) by auto
+  ultimately show ?case using \<open>s = s' \<and> t = 1\<close> by blast
+next
+  case (Assign v a)
+  then have "M =((Aexp_TM idd a);;(tm_cp_until 2 (idd v) {\<box>}))" using while_TM_aux.simps(2) by presburger
+  let ?M1="(Aexp_TM idd a)"
+  let ?M2="(tm_cp_until 2 (idd v) {\<box>})"
+  let ?tps="(IMPminus_state_to_TM_tape_list prog s)"
+  then show ?case proof (cases a)
+    case (A x)
+    then have "?M1= ( atomExp_TM idd x 2)"by simp
+    then show ?thesis sorry
+  next
+    case (Plus x21 x22)
+    then show ?thesis sorry
+  next
+    case (Sub x31 x32)
+    then show ?thesis sorry
+  next
+    case (Parity x4)
+    then show ?thesis sorry
+  next
+    case (RightShift x5)
+    then show ?thesis sorry
+  qed
+next
+  case (Seq prog1 prog2)
+  obtain t1 t2 s'' where "(prog1, s)\<Rightarrow>\<^bsup>t1\<^esup>\<^esup>s''" and  "(prog2, s'')\<Rightarrow>\<^bsup>t-t1\<^esup>\<^esup>s'" and "t1\<le>t" using Seq.prems(2) by auto
+  let ?M1 = "while_TM_aux prog1 idd"
+  let ?M2 = "while_TM_aux prog2 idd"
+  have "(prog1, s)\<Rightarrow>\<^bsup>t1\<^esup>\<^esup>s''" by (simp add: \<open>(prog1, s) \<Rightarrow>\<^bsup> t1 \<^esup>\<^esup> s''\<close>)
+  have r1:"var_set prog1 \<subseteq>var_set (prog1;;prog2)" by fastforce
+  have "(prog1;;prog2)  (idd) \<turnstile> tps \<sim> s" using Seq.prems(4) by blast
+  then have "prog1 (idd) \<turnstile> tps \<sim> s " using r1 tape_list_equiv_IMPminus_state_for_Seq  by blast
+  then obtain tps' where r1:" transforms ?M1 tps ((100::nat) * t1 ^ 4) tps'\<and>
+     prog1 (idd) \<turnstile> tps' \<sim> s'' "  using Seq.IH(1) using Seq.prems(3) \<open>(prog1, s) \<Rightarrow>\<^bsup> t1 \<^esup>\<^esup> s''\<close> by fastforce
+  have r2:"var_set prog2 \<subseteq>var_set (prog1;;prog2)" by fastforce
+  have r3: "inj idd \<and> (\<forall>x\<in>(var_set prog2). (idd x) \<ge>3) " by (simp add: Seq.prems(3))
+  have " prog2 (idd) \<turnstile> tps' \<sim> s''" sorry
+  then obtain tps'' where r2:" transforms ?M2 tps' ((100::nat) * (t-t1) ^ 4) tps''\<and>
+     prog2 (idd) \<turnstile> tps'' \<sim> s' "using  \<open>(prog2, s'')\<Rightarrow>\<^bsup>t-t1\<^esup>\<^esup>s'\<close> using Seq.IH(2) r3 by presburger
+  let ?M = "while_TM_aux (prog1;;prog2) idd"
+  have "?M=?M1;;?M2" by auto
+ 
+  have "length tps =length tps'\<and> length tps'=length tps''" using r1 r2  using length_tps_stable by blast
+(*
 lemma transforms_turing_machine_sequential:
   assumes "transforms M1 tps1 t1 tps2" and "transforms M2 tps2 t2 tps3"
   shows "transforms (M1 ;; M2) tps1 (t1 + t2) tps3"
 *)
+  then have r4:" transforms (?M1;;?M2) tps ((100::nat) * t1 ^ 4+(100::nat) * (t-t1)^ 4) tps''"
+    using  transforms_turing_machine_sequential r1 r2 by blast
+  have r5:"(100::nat) * t1 ^ 4+(100::nat) * (t-t1)^ 4\<le>(100::nat) * (t) ^ 4" using ineq4 \<open>t1 \<le> t\<close>    
+  by (metis distrib_left_numeral le_add_diff_inverse mult_le_mono2)
+  then have r6:" transforms (?M1;;?M2) tps ((100::nat) * t^ 4) tps''"
+  using r4 transforms_monotone by blast
+  have r7:"(prog1;;prog2)  (idd) \<turnstile> tps'' \<sim> s'" sorry
+  show ?case using r7 r6 using Seq.prems(1) by auto
+next
+  case (If x1 prog1 prog2)
+  then show ?case sorry
+next
+  case (While x1 prog)
+  then show ?case sorry
+qed
 
-(*
-definition running_time :: "machine \<Rightarrow> config \<Rightarrow> nat" where
-  "running_time M cfg \<equiv> LEAST t. fst (execute M cfg t) = length M"
-*)
 
-theorem while_TM_in_exp_time:
-  assumes " (com,s) \<Rightarrow>\<^bsup> n \<^esup> t"
-  
-  shows "running_time "
-  "running_time M cfg \<le> 3*n*n"
 
 
 end
